SetTheory/Function.lean
@@ -6,8 +6,47 @@ variable [Zermelo V] {r x y z a b c : V}
 
 /-- A set `f` is a function if all its elements are ordered pairs, and any two pairs of the form
 `⟨x, s⟩, ⟨x, t⟩` in `f` have `s = t`. -/
-structure IsFunction (f : V) extends IsRelation f : Prop where
-  eq : ∀ x s t, opair x s ∈ f → opair x t ∈ f → s = t
+def IsFunction (f : V) :=
+  IsRelation f ∧ ∀ x s t, opair x s ∈ f → opair x t ∈ f → s = t
+
+protected def _root_.BoundedFormula.isFunction (f : α ⊕ Fin n) : BoundedFormula α n :=
+  .and
+    (.isRelation f)
+    -- ∀ x s t u v
+    (.all (.all (.all (.all (.all (.imp
+      -- u = (x, s)
+      (.eqOPair (Sum.inr ⟨n + 3, Nat.lt_add 1⟩)
+        (Sum.inr ⟨n, Nat.lt_add 4⟩) (Sum.inr ⟨n + 1, Nat.lt_add 3⟩))
+      -- v = (x, t)
+      (.imp (.eqOPair (Sum.inr ⟨n + 4, Nat.lt_add 0⟩)
+        (Sum.inr ⟨n, Nat.lt_add 4⟩) (Sum.inr ⟨n + 2, Nat.lt_add 2⟩))
+      -- u ∈ f
+      (.imp (.mem (Sum.inr ⟨n + 3, Nat.lt_add 1⟩)
+        (termSucc (termSucc (termSucc (termSucc (termSucc f))))))
+      -- v ∈ f
+      (.imp (.mem (Sum.inr ⟨n + 4, Nat.lt_add 0⟩)
+        (termSucc (termSucc (termSucc (termSucc (termSucc f))))))
+      -- s = t
+      (.eq (Sum.inr ⟨n + 1, Nat.lt_add 3⟩) (Sum.inr ⟨n + 2, Nat.lt_add 2⟩)))))))))))
+
+@[simp]
+theorem interpret_isFunction {f : α ⊕ Fin n} :
+    Interpret V (.isFunction f) v l ↔ IsFunction (interpretTerm V v l f) := by
+  unfold BoundedFormula.isFunction IsFunction
+  aesop
+
+/-- `f` maps `x` to `y` if `(x, y) ∈ f`. -/
+protected def _root_.BoundedFormula.maps (f x y : α ⊕ Fin n) : BoundedFormula α n :=
+  .exists (.and
+    (.eqOPair (Sum.inr (Fin.last n)) (termSucc x) (termSucc y))
+    (.mem (Sum.inr (Fin.last n)) (termSucc f)))
+
+@[simp]
+theorem interpret_maps {f x y : α ⊕ Fin n} :
+    Interpret V (.maps f x y) v l ↔
+    opair (interpretTerm V v l x) (interpretTerm V v l y) ∈ interpretTerm V v l f := by
+  unfold BoundedFormula.maps
+  simp
 
 /-- A *function* `x ⟶ y` is a relation `f` with domain equal to `x` and range contained in `y`,
 such that if `(a, b), (a, c) ∈ f`, we have `b = c`. -/
@@ -24,6 +63,8 @@ theorem mem_of_mem_dom (f : a ⟶ b) (hx : x ∈ dom f.graph) : x ∈ a :=
 
 theorem mem_dom_of_mem (f : a ⟶ b) (hx : x ∈ a) : x ∈ dom f.graph :=
   by rwa [f.dom_eq]
+
+-- TODO: Are the following definitions even useful?
 
 def apply (f x : V) : V := ⋃ image f {x}
 
@@ -44,7 +85,7 @@ theorem eq_of_opair_mem_graph (f : a ⟶ b) (h : opair x y ∈ f.graph) : y = f 
   · intro h'
     exact ⟨_, h, h'⟩
   · intro ⟨t, ht, ht'⟩
-    cases f.isFunction.eq x y t h ht
+    cases f.isFunction.2 x y t h ht
     exact ht'
 
 theorem opair_mem_graph (f : a ⟶ b) (h : x ∈ a) : opair x (f x) ∈ f.graph := by
@@ -70,7 +111,7 @@ theorem Function.ext {f g : a ⟶ b} (h : ∀ x ∈ a, f x = g x) : f = g := by
   ext x
   constructor
   · intro hx
-    obtain ⟨x, y, rfl⟩ := f.isFunction.isOPair x hx
+    obtain ⟨x, y, rfl⟩ := f.isFunction.1 x hx
     have : x ∈ a := by
       refine mem_of_mem_dom f ?_
       rw [mem_dom_iff]
@@ -79,7 +120,7 @@ theorem Function.ext {f g : a ⟶ b} (h : ∀ x ∈ a, f x = g x) : f = g := by
     rw [hx]
     exact h _ this
   · intro hx
-    obtain ⟨x, y, rfl⟩ := g.isFunction.isOPair x hx
+    obtain ⟨x, y, rfl⟩ := g.isFunction.1 x hx
     have : x ∈ a := by
       refine mem_of_mem_dom g ?_
       rw [mem_dom_iff]
@@ -90,16 +131,13 @@ theorem Function.ext {f g : a ⟶ b} (h : ∀ x ∈ a, f x = g x) : f = g := by
 
 def comp (g : b ⟶ c) (f : a ⟶ b) : a ⟶ c where
   graph := rcomp g.graph f.graph
-  isFunction := {
-    rcomp_isRelation f.isFunction.toIsRelation with
-    eq := by
-      intro x s t hs ht
-      rw [opair_mem_rcomp_iff] at hs ht
-      obtain ⟨u, hgu, hfu⟩ := hs
-      obtain ⟨v, hgv, hfv⟩ := ht
-      cases f.isFunction.eq x u v hfu hfv
-      exact g.isFunction.eq u s t hgu hgv
-  }
+  isFunction := ⟨rcomp_isRelation f.isFunction.1, by
+    intro x s t hs ht
+    rw [opair_mem_rcomp_iff] at hs ht
+    obtain ⟨u, hgu, hfu⟩ := hs
+    obtain ⟨v, hgv, hfv⟩ := ht
+    cases f.isFunction.2 x u v hfu hfv
+    exact g.isFunction.2 u s t hgu hgv⟩
   dom_eq := by
     rw [dom_rcomp, f.dom_eq]
     rw [g.dom_eq]
