SetTheory/Nat.lean
@@ -1,0 +1,195 @@
+import SetTheory.Function
+
+namespace SetTheory
+
+variable [Zermelo V]
+
+/-- `x` is the union of `y` and `z` if `∀ t, t ∈ x ↔ t ∈ y ∨ t ∈ z`. -/
+protected def _root_.BoundedFormula.eqUnion (x y z : α ⊕ Fin n) : BoundedFormula α n :=
+  .all (.iff
+    (.mem (Sum.inr (Fin.last n)) (termSucc x))
+    (.or
+      (.mem (Sum.inr (Fin.last n)) (termSucc y))
+      (.mem (Sum.inr (Fin.last n)) (termSucc z))))
+
+@[simp]
+theorem interpret_eqUnion {x y z : α ⊕ Fin n} :
+    Interpret V (.eqUnion x y z) v l ↔
+    interpretTerm V v l x = interpretTerm V v l y ∪ interpretTerm V v l z := by
+  unfold BoundedFormula.eqUnion
+  rw [ext_iff]
+  simp
+
+/-- `x` is the successor of `y` if `x = y ∪ {y}`. -/
+protected def _root_.BoundedFormula.eqSucc (x y : α ⊕ Fin n) : BoundedFormula α n :=
+  -- ∃ t
+  .exists (.and
+    -- t = {y}
+    (.eqSingleton (Sum.inr (Fin.last n)) (termSucc y))
+    -- x = y ∪ {y}
+    (.eqUnion (termSucc x) (termSucc y) (Sum.inr (Fin.last n)))
+  )
+
+@[simp]
+theorem interpret_eqSucc {x y : α ⊕ Fin n} :
+    Interpret V (.eqSucc x y) v l ↔
+    interpretTerm V v l x = succ (interpretTerm V v l y) := by
+  unfold BoundedFormula.eqSucc succ
+  simp
+
+/-- `x` is the empty set if `∀ y, y ∉ x`. -/
+protected def _root_.BoundedFormula.eqEmpty (x : α ⊕ Fin n) : BoundedFormula α n :=
+  .all (.not (.mem (Sum.inr (Fin.last n)) (termSucc x)))
+
+@[simp]
+theorem interpret_eqEmpty {x : α ⊕ Fin n} :
+    Interpret V (.eqEmpty x) v l ↔ interpretTerm V v l x = ∅ := by
+  unfold BoundedFormula.eqEmpty
+  rw [eq_empty_iff_forall_not_mem]
+  simp
+
+/-- `x` is successor-closed if whenever `t ∈ x`, we have `t ∪ {t} ∈ x`. -/
+protected def _root_.BoundedFormula.succClosed (x : α ⊕ Fin n) : BoundedFormula α n :=
+  .all (.imp
+    -- ∀ t ∈ x
+    (.mem (Sum.inr (Fin.last n)) (termSucc x))
+    -- ∃ u
+    (.exists (.and
+      -- u = succ t
+      (.eqSucc (Sum.inr ⟨n + 1, Nat.lt_add 0⟩) (Sum.inr ⟨n, Nat.lt_add 1⟩))
+      -- u ∈ x
+      (.mem (Sum.inr ⟨n + 1, Nat.lt_add 0⟩) (termSucc (termSucc x)))
+    )))
+
+@[simp]
+theorem interpret_succClosed {x : α ⊕ Fin n} :
+    Interpret V (.succClosed x) v l ↔
+    ∀ y ∈ interpretTerm V v l x, succ y ∈ interpretTerm V v l x := by
+  unfold BoundedFormula.succClosed
+  simp
+
+theorem inductive_iff (x : V) : Inductive x ↔ ∅ ∈ x ∧ ∀ y ∈ x, succ y ∈ x := by
+  constructor
+  · intro h
+    exact ⟨h.empty_mem, h.succ_mem⟩
+  · intro h
+    exact ⟨h.1, h.2⟩
+
+/-- `x` is an inductive set if it contains an empty set and is successor-closed. -/
+protected def _root_.BoundedFormula.isInductive (x : α ⊕ Fin n) : BoundedFormula α n :=
+  .and
+    (.exists (.and
+      (.eqEmpty (Sum.inr (Fin.last n)))
+      (.mem (Sum.inr (Fin.last n)) (termSucc x))))
+    (.succClosed x)
+
+@[simp]
+theorem interpret_isInductive {x : α ⊕ Fin n} :
+    Interpret V (.isInductive x) v l ↔ Inductive (interpretTerm V v l x) := by
+  unfold BoundedFormula.isInductive
+  rw [inductive_iff]
+  simp
+
+/-- `x` is a natural number if it is a member of every inductive set. -/
+protected def _root_.BoundedFormula.isNat (x : α ⊕ Fin n) : BoundedFormula α n :=
+  .all (.imp
+    (.isInductive (Sum.inr (Fin.last n)))
+    (.mem (termSucc x) (Sum.inr (Fin.last n))))
+
+theorem interpret_isNat' {x : α ⊕ Fin n} :
+    Interpret V (.isNat x) v l ↔ ∀ y : V, Inductive y → interpretTerm V v l x ∈ y := by
+  unfold BoundedFormula.isNat
+  simp
+
+/-- The natural numbers. -/
+def ω : V :=
+  sep
+    (.isNat (Sum.inr 0))
+    (fun (i : Empty) => i.elim)
+    Infinity.inductiveSet
+
+theorem mem_ω_iff : n ∈ (ω : V) ↔ ∀ s : V, Inductive s → n ∈ s := by
+  unfold ω
+  simp only [mem_sep_iff, interpret_isNat', interpret_inr, and_iff_right_iff_imp]
+  intro hn
+  exact hn _ Infinity.inductiveSet_inductive
+
+@[simp]
+theorem interpret_isNat {x : α ⊕ Fin n} :
+    Interpret V (.isNat x) v l ↔ interpretTerm V v l x ∈ (ω : V) := by
+  rw [mem_ω_iff, interpret_isNat']
+
+theorem empty_mem_ω : ∅ ∈ (ω : V) := by
+  rw [mem_ω_iff]
+  intro s hs
+  exact hs.empty_mem
+
+theorem succ_mem_ω (hn : n ∈ (ω : V)) : succ n ∈ (ω : V) := by
+  rw [mem_ω_iff] at hn ⊢
+  intro s hs
+  exact hs.succ_mem n (hn s hs)
+
+theorem ω_inductive : Inductive (ω : V) :=
+  ⟨empty_mem_ω, fun _ => succ_mem_ω⟩
+
+def nat_to_ω : Nat → V
+  | 0 => ∅
+  | n + 1 => succ (nat_to_ω n)
+
+/-- The metatheoretic naturals embed in the model `V`. -/
+instance : OfNat V n where
+  ofNat := nat_to_ω n
+
+theorem zero_def : (0 : V) = ∅ := rfl
+
+theorem one_def : (1 : V) = {∅} := by
+  show ∅ ∪ {∅} = {∅}
+  simp
+
+theorem ofNat_succ {n : Nat} : (OfNat.ofNat (n + 1) : V) = succ (OfNat.ofNat n) := rfl
+
+/-- We say that `f` is an *attempt* of the recursion scheme given by the zero case `Z`
+and the successor case `S` if
+* `f` is a function with domain `0 ∈ dom f ∈ ω`;
+* `f 0 = Z`; and
+* `f (succ n) = S (f n)`.
+-/
+structure IsAttempt (f Z S : V) : Prop where
+  isFunction : IsFunction f
+  dom_mem_ω : dom f ∈ (ω : V)
+  zero_mem_dom : 0 ∈ dom f
+  zero_spec : opair 0 Z ∈ f
+  succ_spec (n : V) (hn₁ : n ∈ (ω : V)) (hn₂ : n ∈ dom f) (hn₃ : succ n ∈ dom f) :
+    (succ n) (S (f n)) ∈ f
+
+protected def _root_.BoundedFormula.isAttempt (f Z S : α ⊕ Fin n) : BoundedFormula α n :=
+  .and (.and (.and (.and
+    -- isFunction
+    (.isFunction f)
+    -- dom_mem_ω
+    (.exists (.and
+      -- ∃ d ∈ ω
+      (.isNat (Sum.inr (Fin.last n)))
+      -- ∀ t, t ∈ dom f ↔ t ∈ d
+      (.all (.iff
+        (.memDom (Sum.inr ⟨n + 1, Nat.lt_add 0⟩) (termSucc (termSucc f)))
+        (.mem (Sum.inr ⟨n + 1, Nat.lt_add 0⟩) (Sum.inr ⟨n, Nat.lt_add 1⟩)))))))
+    -- zero_mem_dom
+    (.all (.imp
+      -- ∀ x, x = ∅ → x ∈ dom f
+      (.eqEmpty (Sum.inr (Fin.last n)))
+      (.memDom (Sum.inr (Fin.last n)) (termSucc f)))))
+    -- zero_spec
+    (.all (.imp
+      -- ∀ x, x = ∅ →
+      (.eqEmpty (Sum.inr (Fin.last n)))
+      -- ∃ t
+      (.exists (.and
+        -- t = (x, Z)
+        _
+        -- t ∈ f
+        _)))))
+    -- succ_spec
+    _
+
+end SetTheory
