SetTheory/TransClosure.lean
@@ -1,0 +1,28 @@
+import SetTheory.Function
+
+namespace SetTheory
+/-- A formula with free variables in `α` is a function class for particular choices of free
+variables `v : α → V` if whenever `f a b` and `f a c`, we have `b = c`. -/
+def IsFunctionClass [Zermelo V] (f : BoundedFormula α 2) (v : α → V) : Prop :=
+  ∀ a b c : V,
+    Interpret V f v (fun k => if k = 0 then a else b) →
+    Interpret V f v (fun k => if k = 0 then a else c) →
+    b = c
+
+/-- The axiom of *replacement*.
+If `f` is a function-class and `s` is a set, then the image of `s` under `f` is a set. -/
+class Replacement (V : Type _) [Zermelo V] where
+  replace (f : BoundedFormula α 2) (v : α → V) (hf : IsFunctionClass f v) (s : V) : V
+  mem_replace_iff (a s : V) :
+    a ∈ replace f v hf s ↔ ∃ t ∈ s, Interpret V f v (fun k => if k = 0 then t else a)
+
+/-- The **Zermelo-Fraenkel** axioms of set theory. -/
+class ZF (V : Type _) extends Zermelo V, Replacement V
+
+variable [ZF V]
+
+/-- A set is *transitive* if members of members of the set are members of the set. -/
+def Transitive (x : V) : Prop :=
+  ⋃ x ⊆ x
+
+end SetTheory
